some theory of wh normal forms and determinism of reduction

theories/Untyped.v
@@ -1,20 +1,52 @@
-From MetaCoq.Template Require Import config utils.
-From MetaCoq.PCUIC Require Import PCUICAst PCUICAstUtils
-  PCUICLiftSubst PCUICUnivSubst PCUICEquality PCUICUtils PCUICPosition.
-From MetaCoq.PCUIC Require Export PCUICCumulativitySpec.
-From MetaCoq.PCUIC Require Export PCUICCases PCUICNormal.
+From MetaCoq.PCUIC Require Import PCUICAst PCUICAstUtils PCUICNormal.
+From LogRel Require Import Automation.
 
-Definition whne := whne RedFlags.default empty_global_env.
-Definition whnf := whnf RedFlags.default empty_global_env.
+Notation whne := (whne RedFlags.default empty_global_env).
+Notation whnf := (whnf RedFlags.default empty_global_env).
 Definition emptyName : aname := 
   ltac:(repeat econstructor).
 
+#[global] Hint Constructors PCUICNormal.whne PCUICNormal.whnf : mltt.
+
 Definition eta {A B} (f : A -> B) : f = fun x => f x := eq_refl.
 
-Inductive isType : term -> Type :=
-  | ProdType {na A B} : isType (tProd na A B)
-  | NeType {Γ A}  : whne Γ A -> isType A. 
+Inductive isType Γ : term -> Type :=
+  | ProdType {na A B} : isType Γ (tProd na A B)
+  | NeType {A}  : whne Γ A -> isType Γ A. 
 
-Inductive isFun : term -> Type :=
-  | lamFun {na A t} : isFun (tLambda na A t)
-  | NeFun  { Γ A }  : whne Γ A -> isFun A.
+Inductive isFun Γ : term -> Type :=
+  | lamFun {na A t} : isFun Γ (tLambda na A t)
+  | NeFun  {A}  : whne Γ A -> isFun Γ A.
+
+Lemma isType_whnf Γ t : isType Γ t -> whnf Γ t.
+Proof.
+  induction 1.
+  all: now constructor.
+Qed.
+
+Lemma isFun_whnf Γ t : isFun Γ t -> whnf Γ t.
+Proof.
+  induction 1.
+  all: now constructor.
+Qed.
+
+Lemma nePi Γ na A B : whne Γ (tProd na A B) -> False.
+Proof.
+  intros H.
+  inversion H.
+  apply mkApps_nisApp in H0 as [? _].
+  2: cbn.
+  all: congruence.
+Qed.
+
+Lemma neLambda Γ na A t : whne Γ (tLambda na A t) -> False.
+Proof.
+  intros H.
+  inversion H.
+  1: cbn in * ; congruence.
+  apply mkApps_nisApp in H0 as [? _].
+  2: cbn.
+  all: congruence.
+Qed.
+
+#[global] Hint Resolve nePi neLambda : mltt.
