theories/Automation.v
@@ -1,0 +1,6 @@
+
+Create HintDb mltt.
+#[global] Hint Constants Opaque : mltt.
+#[global] Hint Variables Transparent : mltt.
+
+Ltac mltt := eauto with mltt.
