theories/Generation.v
@@ -1,0 +1,146 @@
+From MetaCoq.PCUIC Require Import PCUICAst PCUICAstUtils.
+From LogRel Require Import Automation MLTTTyping Properties.
+
+Inductive termGenData Γ : term -> term -> Type :=
+  | VarGen n decl :
+      [|- Γ] -> nth_error Γ n = Some decl ->
+      termGenData Γ (tRel n) (lift0 (S n) decl.(decl_type))
+  | ProdGen na A B :
+      [Γ |- A ::: U] ->
+      [Γ,, vass na A |- B ::: U] ->
+      termGenData Γ (tProd na A B) U
+  | LamGen na A B t :
+      [Γ |- A] ->
+      [Γ,, vass na A |- t ::: B] ->
+      termGenData Γ (tLambda na A t) (tProd na A B)
+  | LamApp na f a A B :
+      [Γ |- f ::: tProd na A B] ->
+      [Γ |- a ::: A] ->
+      termGenData Γ (tApp f a) (B{0 := a}).
+
+Lemma termGen Γ t A :
+  [Γ |- t ::: A] ->
+  ∑ A', (termGenData Γ t A') × ((A' = A) + [Γ |- A' ≅ A]).
+Proof.
+  induction 1.
+  1-4: solve 
+    [eexists ; split ; [now econstructor | left ; reflexivity]].
+  destruct IHX as [A' [? [-> | ]]].
+  - eexists. split.
+    1: eassumption.
+    now right.
+  - eexists. split.
+    1: eassumption.
+    right.
+    mltt.
+Qed.  
+
+Inductive termRedGenData Γ : term -> term -> term -> Type :=
+  | AppRedGen na A B t u a :
+      [ Γ |- t ⇒ u ::: tProd na A B] ->
+      [ Γ |- a ::: A ] ->
+    termRedGenData Γ (tApp t a) (tApp u a) (B{0 := a})
+  | BRedGen na A B a t :
+      [ Γ |- A ] -> 
+      [ Γ ,, vass na A |- t ::: B ] ->
+      [ Γ |- a ::: A ] ->
+      termRedGenData Γ (tApp (tLambda na A t) a) (t{0 := a}) (B{0 := a}).
+
+Lemma termRedGen Γ t u A :
+  [Γ |- t ⇒ u ::: A] ->
+  ∑ A', (termRedGenData Γ t u A') × ((A' = A) + [Γ |- A' ≅ A]).
+Proof.
+  induction 1. 
+  1-2: solve 
+    [eexists ; split ; [now econstructor | left ; reflexivity]].
+  destruct IHX as [? [? [-> | ]]].
+  all: eexists ; split ; [eassumption | right ].
+  1: now eassumption.
+  mltt.
+Qed.
+
+Fixpoint fragment (t : term) : bool :=
+  match t with
+    | tRel _ => true
+    | tSort u => eqb Universe.type0 u
+    | tProd _ A B => fragment A && fragment B
+    | tLambda _ A t => fragment t && fragment A
+    | tLetIn _ A t u => fragment u && fragment t && fragment A
+    | tApp t u => fragment t && fragment u
+    | _ => false
+  end.
+
+Lemma fragment_mkApps t l : fragment (mkApps t l) = fragment t && (forallb fragment l).
+Proof.
+  induction l as [|h l' IHt] using list_ind_rev; cbn.
+  - now rewrite andb_true_r.
+  - rewrite mkApps_app, forallb_app ; cbn.
+    rewrite IHt, andb_true_r.
+    now rewrite andb_assoc.
+Qed.
+
+Definition fragment_ctx (Γ : context) : bool :=
+  forallb
+    (fun d => if d.(decl_body) then false else fragment d.(decl_type))
+    Γ.
+
+Lemma fragment_lift k n t : fragment (lift k n t) = fragment t.
+Proof.
+  induction t in k, n |- * ; cbn.
+  all:
+  repeat match goal with
+      | H : forall k n, _ = _ |- _ => rewrite H in * ; cbn in *
+    end.
+  all: reflexivity.
+Qed.
+
+Lemma fragment_subst k t u : fragment t -> fragment u -> fragment (t{k := u}).
+Proof.
+  unfold subst1.
+  induction t in k |- * ; cbn.
+  all:
+    intros ; repeat match goal with
+      | H : is_true (_ && _) |- _ => apply andb_andI in H as []
+      | H : forall k, _ -> _ -> is_true _ |- _ => rewrite H in * ; cbn in *
+    end ; auto.
+  case (k <=? n).
+  1: case (n-k) ; cbn ; [..| intros ? ; rewrite nth_error_nil].
+  2-3: reflexivity.
+  now rewrite fragment_lift.
+Qed.
+
+Lemma wfFrag :
+  (forall Γ : context, [  |- Γ ] -> fragment_ctx Γ)
+  × (forall (Γ : context) (t : term), [Γ |- t] -> fragment_ctx Γ && fragment t)
+    × (forall (Γ : context) (t A : term), [Γ |- t ::: A] -> fragment t && fragment A && fragment_ctx Γ)
+    × (forall (Γ : context) (A B : term), [Γ |- A ≅ B] -> fragment A && fragment B && fragment_ctx Γ)
+        × (forall (Γ : context) (t u A : term),
+          [Γ |- t ≅ u ::: A] -> fragment t && fragment u && fragment A && fragment_ctx Γ).
+Proof.
+  eapply wfInduction ; cbn in * ; intros.
+  2: fold (fragment_ctx Γ).
+  all : intros ;
+    repeat match goal with
+      | H : is_true (_ && _) |- _ => apply andb_andI in H as []
+      | H : is_true _ |- _ => rewrite H in * ; cbn -[fragment_ctx] in *
+    end.
+  all: try reflexivity.
+  2-4: repeat rewrite fragment_subst ; eauto.
+  rewrite fragment_lift.
+  induction Γ in n, H, H0 |- *.
+  - rewrite nth_error_nil in H0. congruence.
+  - destruct n ; cbn in *.
+    all: apply andb_andI in H as [].
+    2: now eapply IHΓ.
+    inversion H0 ; subst ; clear H0.
+    destruct decl as [? []] ; cbn in *.
+    1: congruence.
+    now rewrite H.
+Qed.
+
+Corollary wfTermFrag Γ t A : [Γ |- t ::: A] -> fragment t.
+Proof.
+  intros H.
+  apply wfFrag in H.
+  now repeat apply andb_andI in H as [H _].
+Qed.
