theories/Properties.v
@@ -1,22 +1,5 @@
-From MetaCoq.Template Require Import config utils.
-From MetaCoq.PCUIC Require Import PCUICAst PCUICAstUtils
-  PCUICLiftSubst PCUICUnivSubst PCUICEquality PCUICUtils PCUICPosition.
-From MetaCoq.PCUIC Require Export PCUICCumulativitySpec.
-From MetaCoq.PCUIC Require Export PCUICCases PCUICNormal.
-From LogRel Require Import MLTTTyping Untyped.
-
-Create HintDb mltt.
-#[global] Hint Constants Opaque : mltt.
-#[global] Hint Variables Transparent : mltt.
-
-Ltac mltt := eauto with mltt.
-
-#[global] Hint Constructors wfType wfContext wfTerm convType convTerm : mltt.
-#[global] Hint Constructors termRed typeRed : mltt.
-
-(*Making the non syntax-directed hints more costly*)
-#[global] Remove Hints wfTermConv TermConv termRedConv : mltt.
-#[global] Hint Resolve wfTermConv TermConv termRedConv | 10 : mltt.
+From MetaCoq.PCUIC Require Import PCUICAst.
+From LogRel Require Import Automation Untyped MLTTTyping.
 
 Definition concons_inv {Γ na A} : [|- Γ,, vass na A] -> [|- Γ].
 Proof.
@@ -35,7 +18,7 @@ Definition WFterm {Γ} {t A} :
     [ |- Γ ].
 Proof.
   induction 1 ; mltt.
-Defined.
+Qed.
 
 #[global] Hint Resolve WFterm : mltt.
 
@@ -44,7 +27,7 @@ Definition WFtype {Γ} {A} :
     [ |- Γ ].
 Proof.
     induction 1; mltt.
-Defined.
+Qed.
 
 #[global] Hint Resolve WFtype : mltt.
 
@@ -53,7 +36,7 @@ Definition WFEqTerm {Γ} {t u A} :
     [ |- Γ ].
 Proof.
     induction 1; mltt.
-Defined.
+Qed.
 
 #[global] Hint Resolve WFEqTerm : mltt.
 
@@ -62,7 +45,7 @@ Definition WFEqType {Γ} {A B} :
     [ |- Γ ].
 Proof.
   induction 1 ; mltt.
-Defined.
+Qed.
 
 #[global] Hint Resolve WFEqType : mltt.
 
@@ -71,7 +54,7 @@ Definition redFirstTerm {Γ t u A} :
   [ Γ |- t ::: A ].
 Proof.
   induction 1 ; mltt.
-Defined.
+Qed.
 
 #[global] Hint Resolve redFirstTerm : mltt.
 
@@ -80,7 +63,7 @@ Definition redFirst {Γ A B} :
   [ Γ |- A ].
 Proof.
   induction 1 ; mltt.
-Defined.
+Qed.
 
 #[global] Hint Resolve redFirst : mltt.
 
@@ -89,7 +72,7 @@ Definition redFirstCTerm {Γ t u A} :
   [ Γ |- t ::: A ].
 Proof.
   induction 1 ; mltt.
-Defined.
+Qed.
 
 #[global] Hint Resolve redFirstCTerm : mltt.
 
@@ -98,7 +81,7 @@ Definition redFirstC {Γ A B} :
   [ Γ |- A ].
 Proof.
   induction 1 ; mltt.
-Defined.
+Qed.
 
 #[global] Hint Resolve redFirstC : mltt.
 
@@ -109,13 +92,13 @@ Defined.
   [ Γ |- t ::: A ].
 Proof.
   now intros [].
-Defined. *)
+Qed. *)
 
 (* Definition redFirstCWF {Γ A B} : 
   [ Γ |- A :⇒*: B ] ->
   [ Γ |- A ].
 Proof.
   now intros [].
-Defined. *)
+Qed. *)
 
 
