theories/Reduction.v
@@ -1,25 +1,31 @@
-From MetaCoq.Template Require Import config utils.
-From MetaCoq.PCUIC Require Import PCUICAst PCUICAstUtils
-  PCUICLiftSubst PCUICUnivSubst PCUICEquality PCUICUtils PCUICPosition.
-From MetaCoq.PCUIC Require Export PCUICCumulativitySpec.
-From MetaCoq.PCUIC Require Export PCUICCases PCUICNormal.
-Require Import MLTTTyping Properties.
+From MetaCoq.PCUIC Require Import PCUICAst PCUICAstUtils.
+From LogRel Require Import Automation Untyped MLTTTyping Generation Properties.
+
+(** Inclusion of the various reduction-like *)
 
 Definition RedConvTe {Γ} {t u A : term} :
     [Γ |- t ⇒ u ::: A] -> 
     [Γ |- t ≅ u ::: A].
 Proof.
     induction 1 ; mltt.
-Defined.
+Qed.
 
 #[global] Hint Resolve RedConvTe : mltt.
+
+Corollary termRedFrag Γ t u A : [Γ |- t ⇒ u ::: A] ->
+fragment t && fragment u && fragment A && fragment_ctx Γ.
+Proof.
+  intros.
+  apply wfFrag.
+  mltt.
+Qed.
 
 Definition RedConvTeC {Γ} {t u A : term} :
     [Γ |- t ⇒* u ::: A] -> 
     [Γ |- t ≅ u ::: A].
 Proof.
   induction 1 ; mltt.
-Defined.
+Qed.
 
 #[global] Hint Resolve RedConvTeC : mltt.
 
@@ -28,7 +34,7 @@ Definition RedConvTy {Γ} {A B : term} :
     [Γ |- A ≅ B].
 Proof.
   induction 1 ; mltt.
-Defined.
+Qed.
 
 #[global] Hint Resolve RedConvTy : mltt.
 
@@ -37,9 +43,29 @@ Definition RedConvTyC {Γ} {A B : term} :
     [Γ |- A ≅ B].
 Proof.
   induction 1 ; mltt.
-Defined.
+Qed.
 
 #[global] Hint Resolve RedConvTyC : mltt.
+
+Definition TypeRedWFConv {Γ} {A B} :
+    [Γ |- A :⇒*: B] ->
+    [Γ |- A ≅ B].
+Proof.
+  intros [] ; mltt.
+Qed.
+
+#[global] Hint Resolve TypeRedWFConv : mltt.
+
+Definition RedConvTeWFC {Γ} {t u A} :
+    [Γ |- t :⇒*: u ::: A] ->
+    [Γ |- t ≅ u ::: A].
+Proof.
+  intros [] ; mltt.
+Qed.
+
+#[global] Hint Resolve RedConvTeWFC : mltt.
+
+(** Type conversion for multi-step reduction *)
 
 Definition ClosureConv {Γ} {t u A B} :
     [Γ |- t ⇒* u ::: A] ->
@@ -48,7 +74,7 @@ Definition ClosureConv {Γ} {t u A B} :
 Proof.
   induction 1 ; mltt.
   all: econstructor ; mltt.
-Defined.
+Qed.
 
 #[global] Hint Resolve ClosureConv | 10 : mltt.
 
@@ -59,27 +85,175 @@ Definition TermRedWFConv {Γ} {t u A B} :
 Proof.
   intros [] ?.
   constructor ; mltt.
-Defined. 
+Qed. 
 
 #[global] Hint Resolve TermRedWFConv | 10 : mltt.
 
-Definition TypeRedWFConv {Γ} {A B} :
-    [Γ |- A :⇒*: B] ->
-    [Γ |- A ≅ B].
+(** Whnf do not reduce *)
+
+Lemma whne_nored Γ n u A :
+  whne Γ n -> [Γ |- n ⇒ u ::: A] -> False.
 Proof.
-  intros [] ; mltt.
-Defined.
+  intros ne red.
+  induction red in ne |- *.
+  - inversion ne ; subst.
+    1: easy.
+    eapply mkApps_tApp_inj in H as [-> ->] ; cbn in *.
+    2: easy.
+    apply termRedFrag in red.
+    rewrite fragment_mkApps in red ; cbn in red.
+    now congruence.
+  - inversion ne ; subst ; clear ne.
+    1: now eapply neLambda.
+    eapply mkApps_tApp_inj in H as [H ->] ; cbn in *.
+    2: easy.
+    symmetry in H.
+    apply mkApps_nisApp in H as [].
+    2: cbn.
+    all: congruence.
+  - easy.
+Qed.
 
-#[global] Hint Resolve TypeRedWFConv : mltt.
-
-Definition RedConvTeWFC {Γ} {t u A} :
-    [Γ |- t :⇒*: u ::: A] ->
-    [Γ |- t ≅ u ::: A].
+Lemma whnf_nored Γ n u A :
+  whnf Γ n -> [Γ |- n ⇒ u ::: A] -> False.
 Proof.
-  intros [] ; mltt.
-Defined.
+  intros nf red.
+  induction red in nf |- *.
+  - inversion nf ; subst.
+    2-5:
+      match goal with
+        | H : mkApps _ _ = tApp _ _ |- _ =>
+          apply mkApps_tApp_inj in H as [-> ->]
+      end ; [|easy] ;
+      apply termRedFrag in red ;
+      rewrite fragment_mkApps in red ; cbn in red ;
+      now congruence.
+    eapply whne_nored.
+    1: eassumption.
+    mltt.
+  - inversion nf.
+    2-5:
+      match goal with
+        | H : mkApps _ _ = tApp _ _ |- _ =>
+          apply mkApps_tApp_inj in H as [He _]
+      end ; [|easy] ;
+      symmetry in He ;
+      apply mkApps_nisApp in He as [] ; cbn ; congruence.
+    inversion X ; subst.
+    1: now eapply neLambda.
+    match goal with
+        | H : mkApps _ _ = tApp _ _ |- _ =>
+          apply mkApps_tApp_inj in H as [He _]
+    end ; [|easy] ;
+    symmetry in He ;
+    apply mkApps_nisApp in He as [] ; cbn ; congruence.
+  - easy.
+Qed.
 
-#[global] Hint Resolve RedConvTeWFC : mltt.
+Corollary whnf_nored_ty Γ A B : [Γ |- A ⇒ B] -> whnf Γ A -> False.
+Proof.
+  intros [].
+  eauto using whnf_nored.
+Qed.
+
+Lemma whnf_cred Γ t u A : [Γ |- t ⇒* u ::: A] -> whnf Γ t -> t = u.
+Proof.
+  intros [] ?.
+  1: reflexivity.
+  exfalso.
+  eauto using whnf_nored.
+Qed.
+
+Corollary whnf_cred_ty Γ A B : [Γ |- A ⇒* B] -> whnf Γ A -> A = B.
+Proof.
+  intros [] ?.
+  1: reflexivity.
+  exfalso.
+  now eapply whnf_nored_ty.
+Qed.
+
+(** Determinism of reduction *)
+
+Lemma red_det {Γ t u v A B} :
+  [Γ |- t ⇒ u ::: A] -> [Γ |- t ⇒ v ::: B] ->
+  u = v.
+Proof.
+  intros red red'.
+  induction red in v, B, red' |- *.
+  - eapply termRedGen in red' as [? [d]].
+    inversion d ; subst ; clear d.
+    + f_equal.
+      eauto.
+    + exfalso.
+      eapply whnf_nored.
+      2: eassumption.
+      now econstructor.
+  - eapply termRedGen in red' as [? [d]].
+    inversion d ; subst ; clear d.
+    + exfalso.
+      eapply whnf_nored.
+      2: eassumption.
+      now econstructor.
+    + reflexivity.
+  - easy.
+Qed.
+
+Lemma red_det_ty {Γ A B C} :
+  [Γ |- A ⇒ B] -> [Γ |- A ⇒ C] ->
+  B = C.
+Proof.
+  intros HB HB'.
+  destruct HB, HB'.
+  now eapply red_det.
+Qed.
+
+Lemma nred_cred_det Γ t u u' A A' :
+  [Γ |- t ↘ u ::: A] -> [Γ |- t ⇒* u' ::: A'] ->
+  [Γ |- u' ↘ u ::: A].
+Proof.
+  intros [red whnf] red'.
+  induction red in whnf, A', u', red' |- *.
+  - constructor ; tea.
+    eapply whnf_cred in red' as -> ; tea.
+    now econstructor.
+  - destruct red'.
+    + econstructor.
+      2: mltt.
+      now econstructor.
+    + epose proof (red_det t0 t1) as <-.
+      eapply IHred ; tea. 
+Qed.
+
+Corollary nred_det Γ t u u' A A' :
+  [Γ |- t ↘ u ::: A] -> [Γ |- t ↘ u' ::: A'] ->
+  u = u'.
+Proof.
+  intros red []. eapply nred_cred_det in red as [] ; tea.
+  symmetry.
+  now eapply whnf_cred.
+Qed.
+
+Lemma nred_cred_det_ty Γ A B B' :
+  [Γ |- A ↘ B] -> [Γ |- A ⇒* B'] ->
+  [Γ |- B' ↘ B].
+Proof.
+  intros [red whnf] red'.
+  induction red in whnf, B', red' |- *.
+  - eapply whnf_cred_ty in red' as -> ; tea.
+    mltt.
+  - destruct red'.
+    1: mltt.
+    + now epose proof (red_det_ty t t0) as <-.
+Qed.
+
+Corollary nred_det_ty Γ A B B' :
+  [Γ |- A ↘ B] -> [Γ |- A ↘ B'] ->
+  B = B'.
+Proof.
+  intros red []. eapply nred_cred_det_ty in red as [] ; tea.
+  symmetry.
+  now eapply whnf_cred_ty.
+Qed.
 
 Ltac skip :=
     match goal with
